Encoder proof

src/Lib/Callback/Overrun.v
@@ -23,29 +23,29 @@ Definition callback  : funspec :=
             0 <= computed_size <= Int.max_unsigned;
             0 <= size <= Int.max_unsigned;
             0 <= computed_size + size <= Int.max_unsigned;
-            isptr buf_p)
+            isptr buf_p;
+            if buf_size <? computed_size + size 
+            then buf_size = 0 else True)
       PARAMS (data_p; Vint (Int.repr size); key_p)
       GLOBALS ()
       SEP (data_at Tsh (tarray tuchar (Zlength data)) (map Vint data) data_p;
            data_at Tsh enc_key_s 
-                   (mk_enc_key buf_p buf_size computed_size) 
+                   (mk_enc_key buf_p buf_size computed_size)
                    key_p;
-          if buf_size <? computed_size + size 
+          if buf_size <? computed_size + size
           then emp
-          else memory_block Tsh size (offset_val computed_size buf_p))    
+          else memory_block Tsh size (offset_val computed_size buf_p))
      POST [tint]
       PROP ()
       LOCAL (temp ret_temp Vzero)
       SEP (data_at Tsh (tarray tuchar (Zlength data)) (map Vint data) data_p;
            if buf_size <? computed_size + size 
-           then data_at Tsh enc_key_s 
-                   (mk_enc_key buf_p 0 (computed_size + size))  
-                   key_p
-           else 
-             (data_at Tsh (tarray tuchar size) (map Vint data) 
-                      (offset_val computed_size buf_p) *
-              data_at Tsh enc_key_s 
-                      (mk_enc_key buf_p buf_size (computed_size + size)) key_p)). 
+           then data_at Tsh enc_key_s (mk_enc_key buf_p 0
+                                                  (computed_size + size)) key_p
+           else (data_at Tsh (tarray tuchar size) (map Vint data) 
+                         (offset_val computed_size buf_p) * 
+                 data_at Tsh enc_key_s (mk_enc_key buf_p buf_size 
+                                                   (computed_size + size)) key_p)). 
 
 Definition callback_overrun_spec : ident * funspec :=
   DECLARE _overrun_encoder_cb callback.
@@ -58,19 +58,19 @@ Theorem bool_der_encode : semax_body Vprog Gprog f_overrun_encoder_cb
                                      callback_overrun_spec.
 Proof.
   start_function.
-  destruct (buf_size <? computed_size + size) eqn : Q.
+  destruct (buf_size <? computed_size + size) eqn:S.
   - repeat forward. 
     assert (buf_size < computed_size + size) by (Zbool_to_Prop; eassumption).
     forward_if 
       (PROP ()
-            LOCAL (temp _t'3 (Vint (Int.repr buf_size)); 
-                   temp _t'2 (Vint (Int.repr computed_size));
-                   temp _key key_p; temp _data data_p; 
-                   temp _size (Vint (Int.repr size));
-                   temp _keyp key_p)
-            SEP (data_at Tsh (tarray tuchar (Zlength data)) (map Vint data) data_p;
-                 data_at Tsh enc_key_s 
-                         (mk_enc_key buf_p 0 computed_size) key_p));
+       LOCAL (temp _t'3 (Vint (Int.repr 0)); 
+              temp _t'2 (Vint (Int.repr computed_size));
+              temp _key key_p; temp _data data_p; 
+              temp _size (Vint (Int.repr size));
+              temp _keyp key_p)
+       SEP (data_at Tsh (tarray tuchar (Zlength data)) (map Vint data) data_p;
+            data_at Tsh enc_key_s 
+                    (mk_enc_key buf_p 0 computed_size) key_p));
       repeat (forward || entailer! || nia).    
   - assert (computed_size + size <= buf_size) by (Zbool_to_Prop; eassumption).
     repeat forward.
