src/Primitive/Boolean/VstEnc.v
@@ -78,15 +78,29 @@ Definition bool_der_encode_spec : ident * funspec :=
          buf_p : val, buf_size : Z, computed_size : Z
     PRE [tptr enc_rval_s, tptr type_descriptor_s, tptr tvoid, tint, 
          tuint, tptr cb_type, tptr tvoid]
+    let tag_len := 
+        match evalErrW (Exec.der_write_tags td) [] with 
+        | Some v => encoded v
+        | None => 0
+        end in
+    let size := match evalErrW (bool_encoder td (bool_of_int sptr_val)) [] with
+                | Some v => encoded v
+                | None => 0
+                end in
       PROP (decoder_type td = BOOLEAN_t;
-            isptr(buf_p)) 
+            isptr(buf_p);
+            0 <= buf_size;
+            buf_size <= Int.max_unsigned;
+            0 <= computed_size;
+            computed_size + size  <= Int.max_unsigned;
+            if (buf_size <? computed_size + tag_len) then (buf_size = 0) else True;
+            if (buf_size <? computed_size + size) then (buf_size = 0) else True) 
       PARAMS (res; td_p; sptr_p; Vint (Int.repr tag_mode);
-             Vint (Int.repr tag); cb_p; app_key_p)
+              Vint (Int.repr tag); cb_p; app_key_p)
       GLOBALS ()
-      SEP (
-           (if buf_size <? computed_size + size
-            then emp 
-            else memory_block Tsh size (offset_val computed_size buf_p));
+      SEP (if buf_size <? (computed_size + 2) + 1 (* this is used after dwt execution, so computed_size += 2 *)
+           then emp 
+           else memory_block Tsh 1 (offset_val (computed_size + 2) buf_p);
            data_at_ Tsh enc_rval_s res;
            data_at_ Tsh type_descriptor_s td_p; 
            data_at Tsh tint (Vint sptr_val) sptr_p;
@@ -97,31 +111,36 @@ Definition bool_der_encode_spec : ident * funspec :=
     POST [tvoid]
       PROP ()
       LOCAL ()
-      SEP (let res_val := 
-               match evalErrW (bool_encoder td (bool_of_int sptr_val)) [] with 
-                          | Some v => mk_enc_rval (encoded v) Vzero 
-                          | None => mk_enc_rval (-1) sptr_p end in
+      let res_val := 
+          match evalErrW (bool_encoder td (bool_of_int sptr_val)) [] with 
+                     | Some v => mk_enc_rval (encoded v) Vzero 
+                     | None => mk_enc_rval (-1) sptr_p end in
+      let tags_len := match evalErrW (Exec.der_write_tags td) [] with
+          | Some v => encoded v
+          | None => 0 end in 
+      let arr := match execErrW (bool_encoder td (bool_of_int sptr_val)) [] with 
+         | Some res => res
+         | None => [] end in
+      let size := if Zlength arr =? 0 then tags_len else Zlength arr in
+      SEP (if buf_size <? computed_size + 2 
+           then emp 
+           else data_at Tsh (tarray tuchar 2) (map Vubyte [1%byte; 1%byte]) 
+                        (offset_val computed_size buf_p);
            data_at Tsh enc_rval_s res_val res;
            data_at_ Tsh type_descriptor_s td_p; 
            data_at Tsh tint (Vint sptr_val) sptr_p;
-           (* In the end we're know result, so we don't need size anymore *)
-           let tags_len := 
-               match evalErrW (Exec.der_write_tags td) [] with
-               | Some v => encoded v
-               | None => 0 end in 
-           (let arr := 
-               match execErrW (bool_encoder td (bool_of_int sptr_val)) [] with 
-               | Some res => res
-               | None => [] end in
-           (let size := if Zlength arr =? 0 then tags_len else Zlength arr in
-           (if buf_size <? computed_size + size
-            then data_at Tsh enc_key_s 
-                         (mk_enc_key buf_p 0 (computed_size + size)) app_key_p
-            else (data_at Tsh (tarray tuchar computed_size) (map Vubyte arr) 
-                          (offset_val computed_size buf_p) * 
-                  data_at Tsh enc_key_s 
-                          (mk_enc_key buf_p buf_size (computed_size + size))    
-                          app_key_p))));
+           if buf_size <? computed_size + size
+           then data_at Tsh enc_key_s 
+                        (mk_enc_key buf_p 0 (computed_size + size)) app_key_p
+           else (data_at Tsh (tarray tuchar (size - tags_len)) 
+                         ([Vint 
+                             (Int.zero_ext 8 
+                                           (Int.repr (Byte.unsigned 
+                                                        (last arr (Byte.zero)))))])
+                         (offset_val (computed_size + tags_len) buf_p) * 
+                 data_at Tsh enc_key_s 
+                         (mk_enc_key buf_p buf_size (computed_size + size))    
+                         app_key_p);
            valid_pointer cb_p; 
            func_ptr' callback cb_p).
 
@@ -129,199 +148,220 @@ Definition Gprog := ltac:(with_library prog [der_write_tags_spec;
                                              callback_overrun_spec; 
                                              bool_der_encode_spec]).
 
-Definition if_post1 cb_p sptr_p res bool_p erval_p td_p tag_mode 
-           tag app_key_p td sptr_val cb_spec buf_p buf_size computed_size := 
-  PROP(is_pointer_or_null(cb_p)
-       (* der_write_tags writes 2 tags(bytes) to buffer *)
-       (*computed_size = (computed_size + 2)%Z*))
-  LOCAL(temp _t'6 (Vint (Int.repr 2)); 
-        temp _t'1 (Vint (Int.repr (encoded {| encoded := 2 |}))); 
-        temp _st sptr_p; lvar _bool_value tuchar bool_p;
-        lvar _erval (Tstruct _asn_enc_rval_s noattr) erval_p; 
-        temp __res res; temp _td td_p; temp _sptr sptr_p; 
-        temp _tag_mode (Vint (Int.repr tag_mode)); 
-        temp _tag (Vint (Int.repr tag)); 
-        temp _cb (cb_p); temp _app_key app_key_p) 
-  SEP(data_at_ Tsh type_descriptor_s td_p; 
-      data_at_ Tsh enc_rval_s res; 
-      let arr := match execErrW (Exec.der_write_tags td) [] with
-                 | Some r => r
-                 | None => [] end in
-      let size := Zlength arr in
-      (if buf_size <? computed_size + size
-       then data_at Tsh enc_key_s 
-                    (mk_enc_key buf_p 0 (computed_size + size)) app_key_p
-       else (data_at Tsh (tarray tuchar computed_size) (map Vubyte arr) 
-                     (offset_val computed_size buf_p) * 
-             data_at Tsh enc_key_s 
-                     (mk_enc_key buf_p buf_size (computed_size + size))    
-                     app_key_p));
-      func_ptr' cb_spec (cb_p); 
-      (match (cb_p) with
-       | Vint _ => data_at_ Tsh tuchar bool_p
-       | _ => data_at Tsh tuchar 
-                     (Vubyte (match execErrW (bool_encoder td (bool_of_int sptr_val)) [] with 
-                              | Some v => last v (Byte.repr (-1)) 
-                              | None => (Byte.repr (-1)) 
-                              end)) bool_p end);
-      field_at Tsh (Tstruct _asn_enc_rval_s noattr) (DOT _encoded) 
-               (Vint (Int.repr 2)) erval_p;
-      field_at Tsh (Tstruct _asn_enc_rval_s noattr) (DOT _failed_type) 
-               (default_val (tptr (Tstruct _asn_TYPE_descriptor_s noattr))) 
-               erval_p;
-      field_at Tsh (Tstruct _asn_enc_rval_s noattr) (DOT _structure_ptr) 
-               (default_val (tptr tvoid)) erval_p; 
-      data_at Tsh tint (Vint sptr_val) sptr_p; 
-      valid_pointer (cb_p)).
-
-Definition if_post2 sptr_val app_key_p v_bool_value cb_spec cb_p v_erval 
-           td_p res sptr_p tag_mode tag buf_p buf_size computed_size size := 
-  PROP()
-  LOCAL(temp _t'6 (Vint (Int.repr 2));
-        temp _t'1 (Vint (Int.repr (encoded {| encoded := 2 |}))); 
-        temp _st sptr_p; lvar _bool_value tuchar v_bool_value;
-        lvar _erval (Tstruct _asn_enc_rval_s noattr) v_erval; 
-        temp __res res; temp _td td_p; temp _sptr sptr_p;
-        temp _tag_mode (Vint (Int.repr tag_mode)); 
-        temp _tag (Vint (Int.repr tag)); 
-        temp _cb (cb_p); temp _app_key app_key_p;
-        temp _t'2 (Vint (Int.repr (if (bool_of_int sptr_val) then 255 else 0))))
-  SEP(if buf_size <? computed_size + size 
-      then data_at Tsh enc_key_s (mk_enc_key buf_p 0 computed_size) app_key_p 
-      else data_at Tsh (tarray tuchar 2) (map Vubyte [1%byte; 1%byte]) 
-                   (offset_val computed_size buf_p) * 
-           data_at Tsh enc_key_s (mk_enc_key buf_p buf_size (computed_size + 2)) 
-                   app_key_p; 
-      (if buf_size <? computed_size + size2
-       then emp
-       else memory_block Tsh size2 (offset_val computed_size buf_p));
-      data_at_ Tsh type_descriptor_s td_p; func_ptr' cb_spec cb_p;
-      data_at_ Tsh tuchar v_bool_value;
-      field_at Tsh (Tstruct _asn_enc_rval_s noattr)
-                (DOT _encoded) (Vint (Int.repr 2)) v_erval;
-      field_at Tsh (Tstruct _asn_enc_rval_s noattr)
-                (DOT _failed_type)
-                 (default_val
-                     (tptr (Tstruct _asn_TYPE_descriptor_s noattr)))
-                  v_erval;
-      field_at Tsh (Tstruct _asn_enc_rval_s noattr)
-                (DOT _structure_ptr) (default_val (tptr tvoid))
-                 v_erval; data_at_ Tsh enc_rval_s res;
-      data_at Tsh tint (Vint sptr_val) sptr_p;
-      valid_pointer cb_p).
-
-Definition loop_inv sptr_p v_bool_value v_erval res td_p tag_mode tag cb_p 
-           app_key_p cb_spec sptr_val buf_p buf_size computed_size size :=
-  PROP()
-  LOCAL(temp _t'4 (Vint (Int.repr 2)); 
-        temp _t'6 (Vint (Int.repr 2)); temp _t'1 (Vint (Int.repr 2)); 
-        temp _st sptr_p; lvar _bool_value tuchar v_bool_value;
-        lvar _erval (Tstruct _asn_enc_rval_s noattr) v_erval;
-        temp __res res; temp _td td_p; temp _sptr sptr_p;
-        temp _tag_mode (Vint (Int.repr tag_mode));
-        temp _tag (Vint (Int.repr tag)); temp _cb (cb_p);
-        temp _app_key app_key_p)
-  SEP(data_at_ Tsh type_descriptor_s td_p;
-      data_at_ Tsh enc_rval_s res; 
-      data_at Tsh enc_key_s (mk_enc_key buf_p buf_size computed_size) app_key_p;
-      (if buf_size <? computed_size + size 
-       then emp 
-       else memory_block Tsh 1 (offset_val 2 buf_p));
-      func_ptr' cb_spec (cb_p);
-      data_at Tsh tuchar (Vubyte (byte_of_bool (bool_of_int sptr_val))) v_bool_value;
-      field_at Tsh (Tstruct _asn_enc_rval_s noattr) (DOT _encoded) 
-               (Vint (Int.add (Int.repr 2) (Int.repr 1))) v_erval;
-      field_at Tsh (Tstruct _asn_enc_rval_s noattr) (DOT _failed_type)  
-               (default_val (tptr (Tstruct _asn_TYPE_descriptor_s noattr)))
-               v_erval;
-      field_at Tsh (Tstruct _asn_enc_rval_s noattr) (DOT _structure_ptr)
-               (default_val (tptr tvoid)) v_erval;
-      data_at Tsh tint (Vint sptr_val) sptr_p;
-      valid_pointer (cb_p)).
-
 Theorem bool_der_encode : semax_body Vprog Gprog 
                                      (normalize_function f_BOOLEAN_encode_der
                                                          composites)
                                      bool_der_encode_spec.
 Proof.
   start_function; rename H into DT; rename H0 into Bf_ptr.
+    rename H1 into Bsz; rename H2 into Bsmu; rename H3 into Csz; 
+      rename H4 into Csmu; rename H5 into BsDWT; rename H6 into BsR.
+  rewrite eval_boolean_enc in Csmu by assumption; unfold encoded in Csmu.
+  rewrite Exec.eval_dwt_boolean in BsDWT by assumption; unfold encoded in BsDWT.
+  rewrite eval_boolean_enc in BsR by assumption; unfold encoded in BsR.
   forward.
-  (* TODO specify data array with der_write_tags output *)
   forward_call (td_p, td, 1, tag_mode, 0, tag, cb_p, app_key_p, buf_p, buf_size, 
                 computed_size).
-  
   rewrite Exec.eval_dwt_boolean by assumption; 
     rewrite Exec.exec_dwt_boolean by assumption; unfold encoded.
   unfold_data_at_ v_erval; unfold_data_at (data_at _ _ _ v_erval).
-  forward.
-  forward.
+  repeat forward.
   forward_if; [contradiction|clear H].
-  forward_if (if_post1 cb_p sptr_p res v_bool_value v_erval td_p tag_mode tag 
-                       app_key_p td sptr_val callback buf_p buf_size computed_size); 
-    unfold if_post1.
+  deadvars!.
+  forward_if (
+      PROP ( )
+      LOCAL (temp _st sptr_p;
+             lvar _bool_value tuchar v_bool_value;
+             lvar _erval (Tstruct _asn_enc_rval_s noattr) v_erval; 
+             temp __res res;
+             temp _cb cb_p; temp _app_key app_key_p)
+      SEP (if buf_size <? computed_size + 2 + 1
+           then data_at Tsh enc_key_s (mk_enc_key buf_p 0 (computed_size + 2 + 1)) 
+                        app_key_p
+           else data_at Tsh (tarray tuchar 1) 
+                        ([Vint (Int.zero_ext 8 (Int.repr (Byte.unsigned 
+                                                            (byte_of_bool 
+                                                               (bool_of_int 
+                                                                  sptr_val)))))]) 
+                        (offset_val (computed_size + 2) buf_p) *
+            data_at Tsh enc_key_s (mk_enc_key buf_p buf_size 
+                                              (computed_size + 2 + 1)) app_key_p;
+           let b_v := match execErrW (bool_encoder td (bool_of_int sptr_val)) 
+                                     [] with 
+                      | Some v => last v (Byte.repr (-1)) 
+                      | None => (Byte.repr (-1)) end in
+           match (cb_p) with 
+           | Vint _ => data_at_ Tsh tuchar v_bool_value
+           | _ => data_at Tsh tuchar (Vint (Int.zero_ext 8 (Int.repr (Byte.unsigned b_v)))) v_bool_value 
+           end;
+           data_at_ Tsh type_descriptor_s td_p;
+           func_ptr' callback cb_p;
+           field_at Tsh (Tstruct _asn_enc_rval_s noattr)
+                    (DOT _encoded) (Vint (Int.repr 2)) v_erval;
+           field_at Tsh (Tstruct _asn_enc_rval_s noattr)
+                    (DOT _failed_type)
+                    (default_val
+                       (tptr (Tstruct _asn_TYPE_descriptor_s noattr)))
+                    v_erval;
+           field_at Tsh (Tstruct _asn_enc_rval_s noattr)
+                    (DOT _structure_ptr) (default_val (tptr tvoid))
+                    v_erval;
+           (if buf_size <? computed_size + 2 
+                        then emp
+                        else data_at Tsh (tarray tuchar 2) 
+                                     (map Vubyte [1%byte; 1%byte]) 
+                                     (offset_val computed_size buf_p));
+           data_at_ Tsh enc_rval_s res;
+           data_at Tsh tint (Vint sptr_val) sptr_p;
+           valid_pointer cb_p)).
   * (* if(cb) = true *)
     forward.
     (* bool_value = *st ? 0xff : 0; /* 0xff mandated by DER */ *)
-    forward_if (if_post2 sptr_val app_key_p v_bool_value callback cb_p v_erval 
-                         td_p res sptr_p tag_mode tag buf_p buf_size 
-                         computed_size 2 size); unfold if_post2.
+    forward_if (
+        PROP()
+        LOCAL(temp _t'2 (Vubyte (byte_of_bool (bool_of_int sptr_val)));
+              temp _st sptr_p; 
+              lvar _bool_value tuchar v_bool_value; 
+              lvar _erval (Tstruct _asn_enc_rval_s noattr) v_erval; 
+              temp __res res; temp _cb cb_p; 
+              temp _app_key app_key_p)
+        SEP(if buf_size <? computed_size + 2 + 1
+            then emp
+            else memory_block Tsh 1 (offset_val (computed_size + 2) buf_p);
+            data_at_ Tsh tuchar v_bool_value;
+            if buf_size <? computed_size + 2 
+            then data_at Tsh enc_key_s (mk_enc_key buf_p 0 (computed_size + 2)) 
+                         app_key_p 
+            else data_at Tsh (tarray tuchar 2) (map Vubyte [1%byte; 1%byte]) 
+                         (offset_val computed_size buf_p) * 
+                 data_at Tsh enc_key_s (mk_enc_key buf_p buf_size 
+                                                   (computed_size + 2)) 
+                         app_key_p;
+            data_at_ Tsh type_descriptor_s td_p; 
+            func_ptr' callback cb_p;
+            field_at Tsh (Tstruct _asn_enc_rval_s noattr)
+                     (DOT _encoded) (Vint (Int.repr 2)) v_erval;
+            field_at Tsh (Tstruct _asn_enc_rval_s noattr)
+                     (DOT _failed_type)
+                     (default_val
+                        (tptr (Tstruct _asn_TYPE_descriptor_s noattr)))
+                     v_erval;
+            field_at Tsh (Tstruct _asn_enc_rval_s noattr)
+                     (DOT _structure_ptr) (default_val (tptr tvoid))
+                     v_erval; data_at_ Tsh enc_rval_s res;
+            data_at Tsh tint (Vint sptr_val) sptr_p;
+            valid_pointer cb_p)).
     - (* if(b) = true *)
-      Intros size.
-      forward; unfold if_post2; Exists size; entailer!.
-      unfold bool_of_int.
-      destruct (sptr_val == 0)%int eqn : S; 
-        [eapply int_eq_e in S; contradiction | auto ].
-    - (* if(b) = false *)
-      Intros size.
-      forward; unfold if_post2; Exists size; entailer!.
-    - 
-      Intros size.
       forward.
-      rewrite <-data_at_tuchar_singleton_array_eq.
-      forward_call ([(Int.zero_ext 8 (Int.repr (if bool_of_int sptr_val 
-                                                then 255 
-                                                else 0)))], 
-                    v_bool_value, 1, app_key_p, buf_p, buf_size, computed_size).
       entailer!.
-      cbn.
+      unfold bool_of_int, byte_of_bool, Vubyte;
+        destruct Int.eq eqn:S; [apply int_eq_e in S; congruence| reflexivity].
+    - (* if(b) = false *)
+      forward.
+      entailer!.
+    - forward.
+      deadvars!.
+      rewrite <-data_at_tuchar_singleton_array_eq.
+      freeze L := (data_at Tsh tint (Vint sptr_val) sptr_p)
+                  (data_at_ Tsh enc_rval_s res)
+                  (data_at_ Tsh type_descriptor_s td_p)
+                  (valid_pointer cb_p).
+      forward_call ([(Int.zero_ext 8 
+                                   (Int.repr (Byte.unsigned (byte_of_bool 
+                                                               (bool_of_int 
+                                                                  sptr_val)))))], 
+                    v_bool_value, 1, app_key_p, buf_p, 
+                    buf_size, computed_size + 2).
+      instantiate (1:= [FRZL L; 
+                        field_at Tsh (Tstruct _asn_enc_rval_s noattr) 
+                                 (DOT _encoded) (Vint (Int.repr 2)) v_erval;
+                        field_at Tsh (Tstruct _asn_enc_rval_s noattr) 
+                                 (DOT _failed_type) 
+                                 (default_val (tptr (Tstruct _asn_TYPE_descriptor_s 
+                                                             noattr))) v_erval;
+                        field_at Tsh (Tstruct _asn_enc_rval_s noattr) 
+                                 (DOT _structure_ptr) (default_val (tptr tvoid)) 
+                                 v_erval;
+                        if buf_size <? computed_size + 2 
+                        then emp
+                        else data_at Tsh (tarray tuchar 2) 
+                                     (map Vubyte [1%byte; 1%byte]) 
+                                     (offset_val computed_size buf_p);
+                        func_ptr' callback cb_p]) in (Value of Frame).
+      destruct (buf_size <? computed_size + 2) eqn:K; 
+        cbn; entailer!.
+      cbn in *.
+      replace (computed_size + 3) with (computed_size + 2 + 1) in BsR by lia.
+      repeat split; try lia; assumption.
+      thaw L.
       forward_if; [congruence|].
       ** (* cb() >= 0 *)
-        unfold if_post1; forward.
-         entailer!.
-         destruct cb_p; intuition.
-         rewrite exec_boolean_enc by assumption.
-         unfold bool_of_int.
-         destruct (sptr_val == 0)%int eqn : S; entailer!.
-       (*    try (erewrite <- data_at_tuchar_singleton_array_eq; 
-                entailer!).
-         unfold len; simpl.
-         unfold byte_of_bool.
-         entailer!.
-         normalize.
-         unfold Vubyte.
-         entailer!.
-         erewrite <- data_at_tuchar_singleton_array_eq.
-         entailer!. *)
+        forward.
+        destruct cb_p; intuition.
+        rewrite exec_boolean_enc by assumption.
+        cbn [Zlength map]; rewrite data_at_tuchar_singleton_array_eq.
+        entailer!.
   * (* post if *)
-    forward; unfold if_post1.
+    forward.
     rewrite H; entailer!.
   * (* if(cb) = false *)
     rewrite exec_boolean_enc by assumption.
-    Intros.
-    forward.
-    forward.
-    unfold mk_enc_rval, encoded, last.
-    forward_loop (loop_inv sptr_p v_bool_value v_erval res td_p tag_mode tag
-                                cb_p app_key_p dummy_callback sptr_val); unfold loop_inv.
+    repeat forward.
+    deadvars!.
+    forward_loop (
+        PROP ( )
+           LOCAL (lvar _bool_value tuchar v_bool_value; 
+               lvar _erval (Tstruct _asn_enc_rval_s noattr) v_erval; 
+               temp __res res)
+        SEP (if buf_size <? computed_size + 2 + 1 
+             then data_at Tsh enc_key_s (mk_enc_key buf_p 0 
+                                                    (computed_size + 2 + 1)) 
+                          app_key_p 
+             else data_at Tsh (tarray tuchar 1) 
+                          [Vint (Int.zero_ext 8 (Int.repr (Byte.unsigned 
+                                                             (byte_of_bool  
+                                                                (bool_of_int 
+                                                                   sptr_val)))))] 
+                          (offset_val (computed_size + 2) buf_p) * 
+                  data_at Tsh enc_key_s (mk_enc_key buf_p buf_size 
+                                                    (computed_size + 2 + 1)) 
+                          app_key_p; 
+             match cb_p with 
+             | Vint _ => data_at_ Tsh tuchar v_bool_value 
+             | _ => data_at Tsh tuchar (Vint (Int.zero_ext 8 (Int.repr 
+                                                               (Byte.unsigned 
+                                                                  (last 
+                                                                     [1%byte; 1%byte; 
+                                                                      byte_of_bool 
+                                                                        (bool_of_int sptr_val)] 
+                                                                     (Byte.repr (-1))))))) 
+                           v_bool_value 
+             end; data_at_ Tsh type_descriptor_s td_p; 
+             func_ptr' callback cb_p; 
+             field_at Tsh (Tstruct _asn_enc_rval_s noattr) (DOT _encoded) 
+                      (Vint (Int.repr 2 + Int.repr 1)%int) v_erval; 
+             field_at Tsh (Tstruct _asn_enc_rval_s noattr) (DOT _failed_type) 
+                      (default_val (tptr (Tstruct _asn_TYPE_descriptor_s noattr))) v_erval; 
+             field_at Tsh (Tstruct _asn_enc_rval_s noattr) (DOT _structure_ptr) 
+                      (default_val (tptr tvoid)) v_erval; 
+             if buf_size <? computed_size + 2 
+             then emp 
+             else data_at Tsh (tarray tuchar 2) (map Vubyte [1%byte; 1%byte]) 
+                          (offset_val computed_size buf_p); 
+             data_at_ Tsh enc_rval_s res; 
+             data_at Tsh tint (Vint sptr_val) sptr_p; 
+             valid_pointer cb_p)).
     - entailer!.
-      destruct cb_p; intuition.
-    - 
-      unfold_data_at_ res; unfold_data_at (data_at _ _ _ res).
+    - unfold_data_at_ res; unfold_data_at (data_at _ _ _ res).
       repeat forward.
       rewrite eval_boolean_enc by assumption.
-      unfold mk_enc_rval, encoded, last.
-      unfold_data_at (data_at _ _ _ res).
-      unfold_data_at_  v_erval; unfold_data_at (data_at _ _ _ v_erval).
+      rewrite exec_boolean_enc by assumption.
+      rewrite Exec.eval_dwt_boolean by assumption.
+      unfold_data_at (data_at _ _ _ res); unfold_data_at_ v_erval; 
+        unfold_data_at (data_at _ _ _ v_erval).
+      cbn.
+      destruct cb_p; intuition.
+      replace (computed_size + 3) with (computed_size + 2 + 1) by lia.
       entailer!.
 Qed.
 
